

Gegeben:

$$A = \begin{pmatrix} 0 & 3 & 0 \\ 3 & 0 & 0 \\ 0 & 0 & 3 \end{pmatrix}, X = \begin{pmatrix} 1 \\ 1 \\ 2 \end{pmatrix}$$

Frage:

$$\lambda \quad Ax = \lambda X$$

Problemlösung:

$$Ax = \lambda X \Leftrightarrow (A - \lambda E)X = 0 \Leftrightarrow \begin{pmatrix} 0-\lambda & 3 & 0 \\ 3 & 0-\lambda & 0 \\ 0 & 0 & 3-\lambda \end{pmatrix} \begin{pmatrix} 1 \\ 1 \\ 2 \end{pmatrix} = \begin{pmatrix} 0 \\ 0 \\ 0 \end{pmatrix} \Leftrightarrow$$

$$\Leftrightarrow \begin{pmatrix} (0-\lambda) \cdot 1 + 3 \cdot 1 + 0 \cdot 2 \\ 3 \cdot 1 + (0-\lambda) \cdot 1 + 0 \cdot 1 \\ 0 \cdot 1 + 0 \cdot 1 + (3-\lambda) \cdot 2 \end{pmatrix} = \begin{pmatrix} 0 \\ 0 \\ 0 \end{pmatrix} \Leftrightarrow \begin{pmatrix} (-\lambda) + 3 + 0 \\ 3 + (-\lambda) + 0 \\ 0 + 0 + (-2\lambda + 6) \end{pmatrix} = \begin{pmatrix} 0 \\ 0 \\ 0 \end{pmatrix} \Leftrightarrow$$

$$\Leftrightarrow \begin{pmatrix} -\lambda + 3 \\ -\lambda + 3 \\ -2\lambda + 6 \end{pmatrix} = \begin{pmatrix} 0 \\ 0 \\ 0 \end{pmatrix} \Leftrightarrow$$

$$\Leftrightarrow \begin{cases} -\lambda + 3 = 0 \\ -\lambda + 3 = 0 \\ -2\lambda + 6 = 0 \end{cases} \Leftrightarrow \begin{cases} -\lambda + 3 = 0 \\ -\lambda + 3 = 0 \\ -\lambda + 3 = 0 \end{cases} \Leftrightarrow -\lambda + 3 = 0 \Leftrightarrow$$

$$\Leftrightarrow \lambda = 3$$

Probe:

$$Ax = \begin{pmatrix} 0 & 3 & 0 \\ 3 & 0 & 0 \\ 0 & 0 & 3 \end{pmatrix} \begin{pmatrix} 1 \\ 1 \\ 2 \end{pmatrix} = \begin{pmatrix} 0 \cdot 1 + 3 \cdot 1 + 0 \cdot 2 \\ 3 \cdot 1 + 0 \cdot 1 + 0 \cdot 2 \\ 0 \cdot 1 + 0 \cdot 1 + 3 \cdot 2 \end{pmatrix} = \begin{pmatrix} 0 + 3 + 0 \\ 3 + 0 + 0 \\ 0 + 0 + 6 \end{pmatrix} = \begin{pmatrix} 3 \\ 3 \\ 6 \end{pmatrix} = 3 \begin{pmatrix} 1 \\ 1 \\ 2 \end{pmatrix} = \lambda X$$

Antwort:

$$\lambda = 3 \quad Ax = \lambda X$$